Clean/Circuit/Lawful.lean
@@ -243,7 +243,7 @@ theorem local_length_eq (circuit : Circuit F α) [lawful: ConstantLawfulCircuit 
   rw [Circuit.total_length_eq, final_offset_eq]
 
 theorem bind_local_length (f : Circuit F α) (g : α → Circuit F β)
-  [f_lawful: LawfulCircuit f] [g_lawful : ∀ a : α, LawfulCircuit (g a)] (n : ℕ) :
+  (f_lawful: LawfulCircuit f) (g_lawful : ∀ a : α, LawfulCircuit (g a)) (n : ℕ) :
     ((f >>= g).operations n).local_length = (f.operations n).local_length + ((g (f.output n)).operations (f.final_offset n)).local_length := by
   apply Nat.add_left_cancel (n:=n)
   let fg_lawful : LawfulCircuit (f >>= g) := .from_bind inferInstance inferInstance
